CoqCode/Auxiliaries.v
@@ -1,5 +1,5 @@
 Require Import Metalib.Metatheory.
-Require Import Language.
+Require Import Language Notations.
 Require Import Coq.Program.Equality.
 
 Lemma anno_equal_split :
@@ -20,12 +20,67 @@ Proof.
   rewrite H. reflexivity.
 Qed.
 
-Lemma typing_sub_check :
-  forall (e : trm) (A B : typ),
-    typing nil nil check_mode e A ->
-    sub A B ->
-    typing nil nil check_mode e B.
+
+(*aux lemma for sub_to_app *)
+Lemma toplike_sub_top :
+  forall (A : typ),
+    sub typ_top A -> toplike A.
 Proof.
-  intros e A B Htyp Hsub.
-  induction Htyp.
+  intros A Hsub.
+  induction A.
+  - inversion Hsub.
+  - constructor.
+  - inversion Hsub; subst.
+    constructor. apply IHA2. assumption.
+  - inversion Hsub; subst.
+    constructor.
+    + apply IHA1. assumption.
+    + apply IHA2. assumption.
+Qed.
+
+Lemma toplike_sub_toplike :
+  forall (A B : typ),
+    toplike A ->
+    sub A B ->
+    toplike B.
+Proof.
+  intros A B Htop Hsub.
+  dependent induction Hsub; eauto.
+  - apply tl_arrow. apply IHHsub2. inversion Htop; subst. assumption.
+  - inversion Htop; subst. apply IHHsub. assumption.
+  - inversion Htop; subst. apply IHHsub. assumption.
+Qed.
+
+(* Lemma lambda_sub_check : *)
+(*   forall (e : trm) (A B D : typ), *)
+(*     typing nil nil check_mode (trm_abs e) (typ_arrow A B) -> *)
+(*     sub (typ_arrow A B) (typ_arrow A D) -> *)
+(*     typing nil nil check_mode (trm_abs e) (typ_arrow A D). *)
+(* Proof. *)
+(*   intros e A B D Htyp Hsub. *)
+(*   inversion Htyp; subst. *)
+(*   - assert (Htl: toplike (typ_arrow A D)). *)
+(*     eapply toplike_sub_toplike; eauto 3. *)
+(*     apply typing_top_value; eauto 3. *)
+(*   - eapply typing_abs1. *)
+
+
+(* Version: all value can be checked by toplike *)
+Lemma typing_sub_check :
+  forall (T : ctx) (v : trm) (A B : typ),
+    (* value v -> *)
+    typing T nil check_mode v A ->
+    sub A B ->
+    typing T nil check_mode v B.
+Proof.
+  intros T e A B Htyp Hsub.
+  dependent induction Htyp.
+  - eapply typing_top_value.
+    eapply toplike_sub_toplike; eauto 3.
+  - inversion Hsub; subst.
+    + eapply typing_top_value; eauto 3.
+    + eapply typing_top_value.
+      eapply tl_arrow. apply toplike_sub_top. assumption.
+    + apply typing_abs1 with (L:=L). intros x Hvar.
+      pose proof (H x) as Hx. apply Hx in Hvar.
 Admitted.
