CoqCode/Deterministic.v
@@ -14,7 +14,6 @@ Proof.
   - inversion H_ord.
 Qed.
 
-
 Lemma tred_toplike :
   forall (A : typ),
     toplike A -> forall e1 e2 e1' e2' : trm, typedred e1 A e1' -> typedred e2 A e2' -> e1' = e2'.
@@ -25,22 +24,18 @@ Proof.
     rewrite H_tred1. rewrite H_tred2. reflexivity.
     constructor. constructor. constructor. constructor.
   - inversion H_tred1; subst; eauto 3.
-    + inversion H1.
-    + inversion H3.
-    + inversion H3.
+    + inversion H0.
+    + inversion H0.
+    + inversion H0.
     + inversion H_tred2; subst; eauto 3.
-      * inversion H4.
-      * inversion H8.
-      * inversion H8.
-      * assert (Heq1: (trm_anno p1 D) = (trm_anno p0 D0)).
+      * inversion H0.
+      * inversion H0.
+      * inversion H0.
+      * assert (Heq1: v1 = v0).
         eapply IHHtop1; eauto 3.
-        assert (Heq2: (trm_anno p2 E) = (trm_anno p3 E0)).
+        assert (Heq2: v2 = v3).
         eapply IHHtop2; eauto 3.
-        eapply anno_equal_split in Heq1.
-        destruct Heq1 as [Heq11 Heq12].
-        eapply anno_equal_split in Heq2.
-        destruct Heq2 as [Heq21 Heq22].
-        rewrite Heq11. rewrite Heq12. rewrite Heq21. rewrite Heq22. reflexivity.
+        rewrite Heq1. rewrite Heq2. reflexivity.
   - assert (HAB: toplike (typ_arrow A B)).
     constructor. assumption.
     eapply tred_ord_toplike in H_tred2; eauto.
@@ -79,30 +74,27 @@ Proof.
     inversion Htyp; subst.
     inversion H3; subst. constructor.
   - intros B Htyp.
-    eapply toplike_sub_top in H0.
-    eapply sub_transitivity.
-    constructor. assumption.
+    eapply toplike_sub_top in H.
+    eapply sub_transitivity; eauto 3.
   - intros B0 Htyp.
     inversion Hval; subst; clear Hval.
     inversion Htyp; subst; clear Htyp.
-    inversion H7; subst.
-    apply sub_arrow. assumption. assumption.
-  - intros B0 Htyp.
-    inversion Htyp; subst; clear Htyp.
     inversion H7; subst; clear H7.
-    apply sub_and_l.
-    eapply IHHred. constructor. assumption.
-    inversion H8; subst.
-    + inversion H3.
-    + apply typing_anno. constructor. assumption.
+    eapply sub_arrow; eauto 3.
   - intros B0 Htyp.
+    inversion Hval; subst; clear Hval.
     inversion Htyp; subst; clear Htyp.
-    inversion H7; subst; clear H7.
-    apply sub_and_r.
-    eapply IHHred. constructor. assumption.
-    inversion H8; subst.
-    + inversion H3.
-    + apply typing_anno. constructor. assumption.
+    + apply sub_and_l.
+      eapply IHHred; eauto 3.
+    + apply sub_and_l.
+      eapply IHHred; eauto 3.
+  - intros B0 Htyp.
+    inversion Hval; subst; clear Hval.
+    inversion Htyp; subst; clear Htyp.
+    + apply sub_and_r.
+      eapply IHHred; eauto 3.
+    + apply sub_and_r.
+      eapply IHHred; eauto 3.
 Qed.
 
 Lemma disjoint_value_consistent :
@@ -125,6 +117,16 @@ Proof.
   eapply tred_toplike. apply Htop. apply Hred1. apply Hred2.
 Qed.
 
+Lemma consistent_value_disjoint :
+  forall (A B : typ) (v1 v2 : trm),
+    value v1 -> value v2 ->
+    consistency_spec v1 v2 ->
+    typing nil nil infer_mode v1 A ->
+    typing nil nil infer_mode v2 B ->
+    disjoint_spec A B.
+Proof.
+Admitted.
+
 Lemma tred_determinism :
   forall (v v1 v2 : trm) (A : typ),
     value v -> (exists B, typing nil nil infer_mode v B) ->
@@ -133,65 +135,69 @@ Proof.
   intros v v1 v2 A Hval Htyp Hred1.
   generalize dependent v2.
   induction Hred1.
-  - intros v2 Hred2. inversion Hred2; subst.
+  - intros v2 Hred2.
+    inversion Hred2; subst.
     + reflexivity.
+    + inversion H.
+  - intros v2 Hred2.
+    inversion Hred2; subst; clear Hred2; eauto.
+    + inversion H.
+    + inversion H. contradiction.
+    + symmetry. eapply tred_ord_toplike; eauto.
+    + symmetry. eapply tred_ord_toplike; eauto.
     + inversion H0.
   - intros v2 Hred2.
     inversion Hred2; subst; clear Hred2.
+    + inversion H2. contradiction.
+    + reflexivity.
+  - intros v0 Hred2.
+    inversion Hred2; subst; eauto.
+    + eapply tred_ord_toplike; eauto 3.
+    + eapply IHHred1; eauto.
+      * inversion Hval; assumption.
+      * destruct Htyp. inversion H0; subst.
+        exists A0. assumption.
+        exists A0. assumption.
+    + destruct Htyp.
+      inversion H0; subst.
+      * inversion Hval; subst; clear Hval.
+        assert (Hcons: consistency_spec v1 v2).
+        eapply disjoint_value_consistent; eauto 3.
+        unfold consistency_spec in Hcons.
+        eapply Hcons; eauto 3.
+      * unfold consistency_spec in H10.
+        eapply H10; eauto 3.
+    + inversion H.
+  - intros v0 Hred2.
+    inversion Hred2; subst; eauto.
+    + eapply tred_ord_toplike; eauto 3.
+    + destruct Htyp.
+      inversion H0; subst; eauto.
+      * inversion Hval; subst; clear Hval.
+        assert(Hcons: consistency_spec v1 v2).
+        eapply disjoint_value_consistent; eauto 3.
+        unfold consistency_spec in Hcons.
+        symmetry. eapply Hcons; eauto 3.
+      * unfold consistency_spec in H10.
+        symmetry. eapply H10; eauto 3.
+    + inversion Hval; subst; clear Hval.
+      eapply IHHred1.
+      * assumption.
+      * destruct Htyp. inversion H0; subst.
+        exists B. assumption.
+        exists B. assumption.
+      * assumption.
+    + inversion H.
+  - intros v0 Hred2.
+    inversion Hred2; subst; clear Hred2.
     + inversion H0.
-    + reflexivity.
-    + inversion H0. contradiction.
-    + symmetry. eapply tred_ord_toplike; eauto.
-    + symmetry. eapply tred_ord_toplike; eauto.
-    + inversion H1.
-  - intros v2 Hred2.
-    inversion Hred2; subst; clear Hred2.
-    + inversion H3. contradiction.
-    + reflexivity.
-  - intros v2 Hred2.
-    inversion Hred2; subst; eauto.
-    + eapply tred_ord_toplike; eauto 3.
-    + eapply IHHred1.
-      * constructor. assumption.
-      * destruct Htyp. inversion H3; subst.
-        inversion H14; subst. inversion H4.
-        exists A. eapply typing_anno. constructor. assumption.
-      * assumption.
-    + destruct Htyp. inversion H3; subst. inversion H14; subst; clear H14. inversion H4.
-      assert(Hcons: consistency_spec (trm_anno p1 A) (trm_anno p2 B)).
-      eapply disjoint_value_consistent; eauto 3.
-      unfold consistency_spec in Hcons.
-      eapply Hcons. apply Hred1. apply H12.
-    + inversion H2.
-  - intros v2 Hred2.
-    inversion Hred2; subst; eauto.
-    + eapply tred_ord_toplike; eauto 3.
-    + destruct Htyp. inversion H3; subst. inversion H14; subst; clear H14. inversion H4.
-      assert(Hcons: consistency_spec (trm_anno p1 A) (trm_anno p2 B)).
-      eapply disjoint_value_consistent; eauto 3.
-      unfold consistency_spec in Hcons.
-      symmetry.
-      eapply Hcons. apply H12. apply Hred1.
-    + eapply IHHred1.
-      * constructor. assumption.
-      * destruct Htyp. inversion H3; subst.
-        inversion H14; subst. inversion H4.
-        exists B. eapply typing_anno. constructor. assumption.
-      * assumption.
-    + inversion H2.
-  - intros v2 Hred2.
-    inversion Hred2; subst; clear Hred2.
-    + inversion H4.
-    + inversion H10.
-    + inversion H10.
-    + assert (Heq1: (trm_anno p1 D) = (trm_anno p0 D0)).
+    + inversion H0.
+    + inversion H0.
+    + assert (Heq1: v1 = v3).
       eapply IHHred1_1; eauto 3.
-      assert (Heq2: (trm_anno p2 E) = (trm_anno p3 E0)).
+      assert (Heq2: v2 = v4).
       eapply IHHred1_2; eauto 3.
-      eapply anno_equal_split in Heq1. destruct Heq1 as [Heq11 Heq12].
-      eapply anno_equal_split in Heq2. destruct Heq2 as [Heq21 Heq22].
-      rewrite Heq11. rewrite Heq12. rewrite Heq21. rewrite Heq22.
-      reflexivity.
+      rewrite Heq1. rewrite Heq2. reflexivity.
 Qed.
 
 Lemma tred_value :
@@ -200,6 +206,51 @@ Lemma tred_value :
 Proof.
   intros v v' A Hval Hred.
   induction Hred; eauto.
+  + apply IHHred. inversion Hval; eauto.
+  + apply IHHred. inversion Hval; eauto.
+Qed.
+
+Lemma tred_transitivity : forall (v1 v2 v3 : trm) (A B : typ),
+    value v1 -> typedred v1 A v2 -> typedred v2 B v3 -> typedred v1 B v3.
+Proof.
+  intros v1 v2 v3 A B Hval Hred1 Hred2.
+  generalize dependent v3.
+  generalize dependent B.
+  dependent induction Hred1; eauto.
+  - intros B v3 Hred2. dependent induction Hred2; eauto.
+  - intros B0 v3 Hred2. dependent induction Hred2; eauto.
+    + constructor. assumption. assumption.
+      pose proof (sub_transitivity D B D0) as Hsub.
+      eapply Hsub; eauto 3.
+  - intros B v3 Hred2.
+    inversion Hval; subst; clear Hval.
+    induction Hred2; eauto.
+  - intros B v3 Hred2. inversion Hval; subst; clear Hval.
+    induction Hred2; eauto.
+  - intros B0 v0 Hred2.
+    generalize dependent v0.
+    induction B0; intros v0 Hred2; eauto.
+    + inversion Hred2; subst; clear Hred2; eauto.
+    + inversion Hred2; subst; clear Hred2; eauto.
+    + inversion Hred2; subst; clear Hred2; eauto.
+    + inversion Hred2; subst; clear Hred2; eauto.
+Qed.
+
+Lemma tred_consistency :
+  forall (v v1 v2 : trm) (A B C : typ),
+    value v -> typing nil nil infer_mode v C ->
+    typedred v A v1 ->
+    typedred v B v2 ->
+    consistency_spec v1 v2.
+Proof.
+  intros v v1 v2 A B C Hval Htyp Hred1 Hred2.
+  unfold consistency_spec.
+  intros D v1' v2' Hred1' Hred2'.
+  assert (Htrans1: typedred v D v1').
+  eapply tred_transitivity. apply Hval. apply Hred1. apply Hred1'.
+  assert (Htrans2: typedred v D v2').
+  eapply tred_transitivity. apply Hval. apply Hred2. apply Hred2'.
+  eapply tred_determinism; eauto 3.
 Qed.
 
 Lemma tred_typing :
@@ -210,10 +261,42 @@ Lemma tred_typing :
     (exists (C : typ), typing nil nil infer_mode v' C).
 Proof.
   intros v v' A Hval Htyp Hred.
-  induction Hred; eauto.
+  induction Hred.
+  - exists typ_int. constructor; eauto 3.
+  - exists typ_top. constructor; eauto 3.
   - destruct Htyp.
-    inversion H2; subst. inversion H7; subst.
-    exists (typ_arrow A D). apply typing_anno; eauto 3.
+    inversion H2; subst.
+    inversion H7; subst.
+    exists (typ_arrow A D).
+    eapply typing_anno; eauto 3.
+    (* so we need checked subsumption here *)
+    assert (Hsub: sub (typ_arrow A B) (typ_arrow A D)).
+    apply sub_arrow. apply sub_reflexivity. assumption.
+    eapply typing_sub_check. apply H8. apply Hsub.
+  - apply IHHred. inversion Hval; subst. assumption.
+    destruct Htyp. inversion H0; subst.
+    + exists A0. assumption.
+    + exists A0. assumption.
+  - apply IHHred. inversion Hval; subst. assumption.
+    destruct Htyp. inversion H0; subst.
+    + exists B. assumption.
+    + exists B. assumption.
+  - assert (Htypl: exists (D : typ), typing nil nil infer_mode v1 D).
+    apply IHHred1. assumption. assumption.
+    assert (Htypr: exists (E : typ), typing nil nil infer_mode v2 E).
+    apply IHHred2. assumption. assumption.
+    destruct Htypl. destruct Htypr.
+    assert(Hval1: value v1). eapply tred_value. apply Hval. apply Hred1.
+    assert(Hval2: value v2). eapply tred_value. apply Hval. apply Hred2.
+    exists (typ_and x x0). apply typing_merge_value; eauto 3.
+    (* well typed value *)
+    destruct Htyp.
+    eapply tred_consistency.
+    + apply Hval.
+    + apply H1.
+    + apply Hred1.
+    + apply Hred2.
+Qed.
 
 Lemma papp_determinism :
   forall (v1 v2 e1 e2 : trm),
@@ -224,19 +307,67 @@ Lemma papp_determinism :
 Proof.
   intros v1 v2 e1 e2 Hval1 Hval2 Htyp1 Htyp2 Hp1.
   generalize dependent e2.
-  induction Hp1.
+  dependent induction Hp1.
   - intros e2 Hp2. inversion Hp2. reflexivity.
   - intros e2 Hp2. inversion Hp2. reflexivity.
   - intros e2 Hp2. inversion Hp2; subst.
     assert (Hequal: v' = v'0).
     eapply tred_determinism; eauto 3.
     rewrite Hequal. reflexivity.
-  - intros e2 Hp2. inversion Hp2; subst; clear Hp2.
-    apply IHHp1.
-    + eapply tred_value. apply Hval1. apply H0.
-    + apply Hval2.
+  - intros e2 Hp2.
+    apply IHHp1; eauto.
+    + eapply tred_value. apply Hval1. apply H2.
+    + eapply tred_typing. apply Hval1. apply Htyp1. apply H2.
     +
+      dependent destruction H0.
+      dependent destruction H1.
+      * dependent destruction H2.
 
+      inversion H1; subst.
+Admitted.
+
+Lemma app_check_typing :
+  forall (e1 e2 : trm) (A : typ),
+    typing nil nil check_mode (trm_app e1 e2) A ->
+    (exists B, typing nil nil infer_mode e1 B) /\
+    (exists C, typing nil nil infer_mode e2 C).
+Proof.
+Admitted.
+
+Lemma value_cannot_step_further :
+  forall (v : trm),
+    value v -> forall (e : trm), not (step v e).
+Proof.
+  intros v Hval.
+  induction v.
+  - inversion Hval.
+  - inversion Hval.
+  - inversion Hval.
+  - inversion Hval.
+  - unfold not. intros. inversion H.
+  - inversion Hval.
+  - inversion Hval; subst.
+    intros. unfold not. intros.
+    inversion H; subst.
+    + eapply IHv1; eauto 3.
+    + eapply IHv2; eauto 3.
+  - inversion Hval; subst; clear Hval.
+    induction H0.
+    + intros. unfold not. intros.
+      inversion H; subst.
+      * inversion H2.
+      * apply H2. constructor. constructor.
+    + intros. unfold not. intros.
+      inversion H; subst.
+      * inversion H2.
+      * apply H2. constructor. constructor.
+    + intros. unfold not. intros.
+      inversion H; subst; clear H.
+      Focus 2.
+      * apply H2. constructor. constructor.
+      * (* that's the problem *)
+        inversion H4; subst.
+Admitted.
 
 Lemma step_determinism :
   forall (e e1 e2 : trm) (A : typ),
@@ -250,6 +381,10 @@ Proof.
   - intros A Htyp e2 Hred2.
     inversion Hred2; subst.
     reflexivity.
-  - intros A0 Htyp e2 Hred2.
+  - intros A Htyp e2 Hred2.
     inversion Hred2; subst.
-Admitted.
+    apply app_check_typing in Htyp. destruct Htyp as [Htyp1 Htyp2].
+    + eapply papp_determinism.
+      apply H. apply H0.
+      apply Htyp1. apply Htyp2. apply H1. apply H7.
+    + (* value cannot step further *)
